steel/formats/spec/Zeta.Formats.Aux.Application_key.Low.fsti
@@ -8,3 +8,4 @@ open LowParse.Low.Base
 val application_key_validator: validator application_key_parser
 val application_key_jumper: jumper application_key_parser
 val application_key_reader: leaf_reader application_key_parser
+val application_key_lserializer: serializer32 application_key_serializer
